WIP for prooving well_justified jctc6 with a candidate execution

jctc6.thy
@@ -1,5 +1,6 @@
 theory jctc6
-  imports EventStructures String Relation Transitive_Closure 
+  imports EventStructures ExampleEventStructures 
+          String Relation Transitive_Closure 
 begin
 
 definition jctc6 :: "nat event_structure" where
@@ -131,16 +132,172 @@ theorem jctc_isValid: "isValidES jctc6"
 thm "justifies_event.induct"
 thm "justifies_event.cases"
   
-theorem "\<exists>C . well_justified jctc6 C \<and> {2, 5} \<subseteq> C"
-  apply(simp add: well_justified_def)
-  apply(simp add: jctc_isValid)
-  apply(simp add: justified_def ae_justifies_star_def ae_justifies_def)
-  apply(simp add: justifies_config_star_inf_def justifies_config_inf_def)
-  apply(simp add: justifies_config_def)
-  apply(induct rule: justifies_event.cases)
-        apply auto[1]
-       apply simp
-          apply auto[1]
-         apply simp
+(* Possibly not very useful.
+inductive aejI :: "'a config \<Rightarrow>'a event_structure \<Rightarrow> 'a config \<Rightarrow> bool" where
+AEJ: "\<lbrakk> \<forall>C' . C \<lesssim>\<^sup>*\<^bsub>es\<^esub> C'; \<exists>C'' . C' \<lesssim>\<^sup>*\<^bsub>es\<^esub> C'' \<and> C'' \<lesssim>\<^bsub>es\<^esub> D \<rbrakk> \<Longrightarrow> aejI C es D"
+
+lemma "aejI C es D \<Longrightarrow> ae_justifies C es D"
+  apply(simp add: ae_justifies_def)
+  apply(simp add: aejI.simps)
   oops
     
+lemma "ae_justifies C es D \<Longrightarrow> aejI C es D"
+  apply(simp add: ae_justifies_def)
+  apply(simp add: aejI.simps)
+  apply auto
+    try
+*)
+definition jctc6_exec:: "nat set" where
+  "jctc6_exec \<equiv> {1,2,3,5,6}"
+
+definition jctc6_C2:: "nat set" where
+  "jctc6_C2 \<equiv> {1,2,3}"
+  
+lemma ae_justifies_refl: "C \<lesssim>\<^sup>*\<^bsub>es\<^esub> C"
+  apply(simp add: justifies_config_star_inf_def)
+  done
+    
+theorem jctc6_reads: "(getMemAction (label_function jctc6 r) = R) = (r \<in> {4,7,2,5})"
+  apply(simp add:jctc6_def)
+  done   
+  
+lemma foo: "{} \<lesssim>\<^sup>*\<^bsub>es\<^esub> C \<Longrightarrow> ({}, C) \<in> justifies_config jctc6"
+  apply(simp add: justifies_config_star_inf_def)
+  apply(simp add: justifies_config_subset_def)
+  
+  oops
+        
+lemma rtrancl_eq_Id_trancl: "r\<^sup>* = Id \<union> r\<^sup>+"
+  by (simp add: Nitpick.rtrancl_unfold Un_commute)
+  
+  
+-- {* For every step of adding something to C' we have that the previous steps are included, so any
+      "dependants" remain.
+      Mark: in the final step (C_0,C') , all reads in C' are justified by C_0, and C_0 is a subset,
+      so all reads in C' are justified by writes in C'. *}
+lemma just_star_imp_just: "{} \<lesssim>\<^sup>*\<^bsub>es\<^esub> C' \<Longrightarrow> C' \<lesssim>\<^bsub>es\<^esub> C'"
+  apply(simp add: justifies_config_star_inf_def) 
+  apply(simp add: rtrancl_eq_Id_trancl)
+  apply(case_tac "{}=C'")                    
+   apply(simp_all)
+   apply(rule emptyESJustEmptyES)
+  apply(simp add: trancl_unfold_right)
+    apply(simp add: justifies_config_subset_def justifies_config_def)
+      
+  sorry
+  
+lemma not_read_6: "\<not> (getMemAction (label_function jctc6 6) = R)"
+  apply(simp add: jctc6_def)
+  done
+    
+lemma write_add_justified: (*"{} \<lesssim>\<^sup>*\<^bsub>es\<^esub> C \<Longrightarrow> 6 \<notin> C' \<and> 8 \<notin> C' \<Longrightarrow> 5 \<in> C \<Longrightarrow> C \<lesssim>\<^sup>*\<^bsub>jctc6\<^esub> C \<union> {6} \<and> (C, C \<union> {6}) \<in> justifies_config jctc6"*)
+  "{} \<lesssim>\<^sup>*\<^bsub>jctc6\<^esub> C' \<Longrightarrow>
+          6 \<notin> C' \<and> 8 \<notin> C' \<Longrightarrow>
+          5 \<in> C' \<Longrightarrow>
+          C' \<lesssim>\<^sup>*\<^bsub>jctc6\<^esub> insert 6 C' \<and>
+          (insert 6 C', jctc6_C2) \<in> justifies_config jctc6"
+  apply (simp add: justifies_config_def)
+  apply(rule conjI)
+  apply(insert just_star_imp_just [where es=jctc6, where C'=C'])
+    apply(simp)
+  apply(simp add: justifies_config_star_inf_def justifies_config_subset_def justifies_config_inf_def)
+  apply(rule r_into_rtrancl)
+  apply(simp)
+  apply(rule conjI)
+    apply(auto)[1]
+  apply (simp add: justifies_config_def)
+   apply(simp add: not_read_6)
+    apply(auto)[1]
+       apply(rule ballI)
+    apply(rule impI)
+  apply(auto simp add: jctc6_def jctc6_C2_def)
+  done
+    
+text {* We want to case split on C', if C' contains a write from which we can justify 2 then we're 
+good and don't need to add anything to C''. Otherwise we need to add a write like 6 or 8. 
+There's no move for C' which doesn't allow adding 6 or 8 to the C'' set. *}
+theorem round_1: "({}, jctc6_C2) \<in> {(c\<^sub>1, c\<^sub>2). c\<^sub>1 \<sqsubseteq>\<^bsub>jctc6\<^esub> c\<^sub>2}"
+  apply(simp add: ae_justifies_subset_def ae_justifies_def)
+  apply (rule allI)
+  apply(rule impI)
+  apply(case_tac "6 \<in> C' \<or> 8 \<in> C'")
+      apply(rule_tac x=C' in exI)
+    -- {* We have the cases for C' now. Let's dispatch the first where we don't need to add 
+          anything to C''*}
+    -- {* When 6 is in C', we can pick C'' = C' and always add 2 to D *}
+    apply(simp add: ae_justifies_refl justifies_config_inf_def justifies_config_def)
+   apply(simp add: jctc6_reads jctc6_C2_def)
+    
+   -- {* These steps are required to prune the proof state back *}
+   apply(rule conjI)
+    apply(auto)[1]
+   apply(rule conjI)
+    apply(erule disjE)
+    
+    -- {* This handles the 6 \<in> C'' case. 6 can justify 2 so we're good to proceed. *}
+    apply(rule_tac x=6 in bexI)
+     apply(simp add: jctc6_def)
+     apply(assumption)
+    
+    -- {* This handles the 8 \<in> C'' case. 8 can justify 2 so we're good to proceed. *}
+    apply(rule_tac x=8 in bexI)
+     apply(simp add: jctc6_def)
+    apply(assumption)
+    
+    apply auto[1]
+    -- {* This is the 6 in C' case done \o/ *}
+    
+    
+  apply(case_tac "5 \<in> C'")
+   apply(rule_tac x="C'\<union>{6}" in exI)
+   apply(simp add: write_add_justified)
+    
+  -- {* If 5 is not in C' we can add 7 and 8 as they're not in conflict. This gets us towards our 
+        goal. Adding 7 is justified by the init, and adding 8 is justified because 8 is a write. *}
+  apply(rule_tac x="C'\<union>{7,8}" in exI)
+    
+
+    sorry
+
+lemma C1_subset_exec: "jctc6_C2 \<subseteq> jctc6_exec"
+  apply(auto simp add: jctc6_C2_def jctc6_exec_def)  
+  done
+    
+text {* Similar to the previous argument, whatever the opponent picks in C' we can always add a WA1 
+either with event 6 or 8. If 6 or 8 are in C' we can pick C'' = C' and have D, otherwise we must add
+one of them to C'' to get D *}
+theorem round_2: "(jctc6_C2, jctc6_exec) \<in> {(c\<^sub>1, c\<^sub>2). c\<^sub>1 \<sqsubseteq>\<^bsub>jctc6\<^esub> c\<^sub>2}"
+  apply(simp add: ae_justifies_def)
+  apply(cases "6 \<in> C' \<or> 8 \<in> C'")
+  sorry
+    
+lemma refl2: "(a, b) \<in> r \<and> (b, c) \<in> r \<Longrightarrow> (a, c) \<in> r\<^sup>*"
+  apply auto
+  done
+
+theorem rounds: "({}, jctc6_C2) \<in> {(c\<^sub>1, c\<^sub>2).  c\<^sub>1 \<sqsubseteq>\<^bsub>jctc6\<^esub> c\<^sub>2} \<and>
+                 (jctc6_C2, jctc6_exec) \<in> {(c\<^sub>1, c\<^sub>2). c\<^sub>1 \<sqsubseteq>\<^bsub>jctc6\<^esub> c\<^sub>2} \<Longrightarrow>
+                 ({}, jctc6_exec) \<in> {(c\<^sub>1, c\<^sub>2).  c\<^sub>1 \<sqsubseteq>\<^bsub>jctc6\<^esub> c\<^sub>2}\<^sup>*"
+  apply (rule refl2)
+  apply auto
+  done
+
+theorem jctc6_game: "{} \<sqsubseteq>\<^sup>*\<^bsub>jctc6\<^esub> jctc6_exec"
+  apply(simp add: ae_justifies_subset_star_def)
+  apply(rule rounds)
+  apply(rule conjI)
+  apply(rule round_1)
+  apply(rule round_2)
+  done
+
+  
+theorem "well_justified jctc6 jctc6_exec \<and> {2, 5} \<subseteq> jctc6_exec"
+  apply(simp add: well_justified_def)
+  apply(simp add: jctc_isValid)
+  apply(auto)
+     defer defer
+     apply(simp add: jctc6_exec_def)
+    apply(simp add: jctc6_exec_def)
+   apply(simp add: justified_def jctc6_reads jctc6_exec_def jctc6_def)
+  apply(simp add: jctc6_game)
+  done
